theories/base_logic/lib/invariants.v
@@ -149,7 +149,7 @@ Section inv.
     ↑N ⊆ E → inv N P ={E,E∖↑N}=∗ ▷ P ∗ ∀ E', ▷ P ={E',↑N ∪ E'}=∗ True.
   Proof.
     iIntros (?) "Hinv".
-    iPoseProof (inv_open (↑ N) N P with "Hinv") as "H"; first done.
+    iPoseProof (inv_open (↑ N) N with "Hinv") as "H"; first done.
     rewrite difference_diag_L.
     iPoseProof (fupd_mask_frame_r _ _ (E ∖ ↑ N) with "H") as "H"; first set_solver.
     rewrite left_id_L -union_difference_L //. iMod "H" as "[$ H]"; iModIntro.
